cleanups

src/Init/Data/Range/Polymorphic/Basic.lean
@@ -10,79 +10,45 @@ import Init.Data.Range.Polymorphic.RangeIterator
 
 open Std.Iterators
 
+namespace Std.PRange
+
+/--
+Internal function that constructs an iterator for a `PRange`. This is an internal function.
+Use `PRange.iter` instead, which requires importing `Std.Data.Iterators`.
+-/
 @[always_inline, inline]
-def PRange.iterInternal [UpwardEnumerable α] [BoundedUpwardEnumerable sl α]
-    (r : PRange ⟨sl, su⟩ α) : Iter (α := Types.RangeIterator su α) α :=
+def Internal.iter [UpwardEnumerable α] [BoundedUpwardEnumerable sl α]
+    (r : PRange ⟨sl, su⟩ α) : Iter (α := RangeIterator su α) α :=
   ⟨⟨BoundedUpwardEnumerable.init? r.lower, r.upper⟩⟩
 
+/--
+Returns the number of elements contained in the given range, given that ranges of the given
+type and shape support this function.
+-/
 @[always_inline, inline]
-def PRange.size [UpwardEnumerable α] [BoundedUpwardEnumerable sl α]
+def size [UpwardEnumerable α] [BoundedUpwardEnumerable sl α]
     [SupportsUpperBound su α] (r : PRange ⟨sl, su⟩ α)
-    [IteratorSize (Types.RangeIterator su α) Id] : Nat :=
-  r.iterInternal.size
+    [IteratorSize (RangeIterator su α) Id] : Nat :=
+  PRange.Internal.iter r |>.size
 
+/--
+Returns the elements of the given range as a list in ascending order, given that ranges of the given
+type and shape support this function and the range is finite.
+-/
 @[always_inline, inline]
-def PRange.toList [UpwardEnumerable α] [BoundedUpwardEnumerable sl α]
+def toList [UpwardEnumerable α] [BoundedUpwardEnumerable sl α]
     [SupportsUpperBound su α]
     (r : PRange ⟨sl, su⟩ α)
-    [Iterator (Types.RangeIterator su α) Id α] [Finite (Types.RangeIterator su α) Id]
-    [IteratorCollect (Types.RangeIterator su α) Id Id] : List α :=
-  r.iterInternal.toList
-
--- instance [UpwardEnumerable α] [HasRange shape α] [BoundedUpwardEnumerable shape α]
---     [ForIn' m (Iter (α := Types.RangeIterator shape α) α) α inferInstance] :
---     ForIn' m (PRange shape α) α where
---   forIn r := forIn r.iter
+    [Iterator (RangeIterator su α) Id α] [Finite (RangeIterator su α) Id]
+    [IteratorCollect (RangeIterator su α) Id Id] : List α :=
+  PRange.Internal.iter r |>.toList
 
 section Iterator
 
--- theorem Range.SuccIterator.succ?_eq_some_of_isPlausibleSuccessorOf [Succ? α] [LE α] [DecidableLE α]
---     {it' it : Iter (α := Types.RangeIterator α inferInstance P) α}
---     [Finite (Types.RangeIterator α inferInstance P) Id]
---     (h' : it'.IsPlausibleSuccessorOf it) :
---     Succ?.succ? 1 it.internalState.next = some it'.internalState.next :=
---   h' |>
---     TakeWhile.isPlausibleSuccessorOf_inner_of_isPlausibleSuccessorOf |>
---     RepeatIterator.Monadic.next_eq_some_of_isPlausibleSuccessorOf
-
-private theorem RangeIterator.isPlausibleIndirectOutput_iff.aux
-    [UpwardEnumerable α] [BoundedUpwardEnumerable sl α] [SupportsLowerBound sl α]
-    [SupportsUpperBound su α] [LawfulUpwardEnumerable α] [LawfulUpwardEnumerableLowerBound sl α]
-    {r : PRange ⟨sl, su⟩ α} {it : Iter (α := Types.RangeIterator su α) α} {a : α}
-    (h : ∃ next, it.internalState.next = some next ∧ SupportsLowerBound.IsSatisfied r.lower next)
-    (h' : it.IsPlausibleIndirectOutput a)
-    (hu : it.internalState.upperBound = r.upper) :
-    a ∈ r := by
-  induction h'
-  case direct it out h' =>
-    simp only [Types.RangeIterator.isPlausibleOutput_iff, hu] at h'
-    obtain ⟨next, hn, hl⟩ := h
-    simp only [h'.1, Option.some.injEq] at hn
-    cases hn
-    exact ⟨hl, h'.2⟩
-  case indirect it it' out  hs ho ih =>
-    rw [Types.RangeIterator.isPlausibleSuccessorOf_iff] at hs
-    obtain ⟨next, hn, h₁, h₂, hs⟩ := hs
-    apply ih
-    · rw [← hs] at hu
-      have ho' := Types.RangeIterator.isSome_next_of_isPlausibleIndirectOutput ho
-      rw [Option.isSome_iff_exists] at ho'
-      obtain ⟨a, ha⟩ := ho'
-      rw [ha] at h₂
-      refine ⟨a, ha, ?_⟩
-      apply LawfulUpwardEnumerableLowerBound.isSatisfied_of_le r.lower next a
-      · obtain ⟨_, hn', hl⟩ := h
-        simp only [hn] at hn'
-        cases hn'
-        exact hl
-      · refine ⟨1, ?_⟩
-        simp [LawfulUpwardEnumerable.succMany?_succ, LawfulUpwardEnumerable.succMany?_zero, h₂]
-    · simp [*]
-
-theorem RangeIterator.isPlausibleIndirectOutput_iff'
+theorem RangeIterator.isPlausibleIndirectOutput_iff
     [UpwardEnumerable α] [SupportsUpperBound su α]
     [LawfulUpwardEnumerable α] [LawfulUpwardEnumerableUpperBound su α]
-    {it : Iter (α := Types.RangeIterator su α) α} {out : α} :
+    {it : Iter (α := RangeIterator su α) α} {out : α} :
     it.IsPlausibleIndirectOutput out ↔
       ∃ n, it.internalState.next.bind (UpwardEnumerable.succMany? n ·) = some out ∧
         SupportsUpperBound.IsSatisfied it.internalState.upperBound out := by
@@ -90,10 +56,10 @@ theorem RangeIterator.isPlausibleIndirectOutput_iff'
   · intro h
     induction h
     case direct h =>
-      rw [Types.RangeIterator.isPlausibleOutput_iff] at h
+      rw [RangeIterator.isPlausibleOutput_iff] at h
       refine ⟨0, by simp [h, LawfulUpwardEnumerable.succMany?_zero]⟩
     case indirect h _ ih =>
-      rw [Types.RangeIterator.isPlausibleSuccessorOf_iff] at h
+      rw [RangeIterator.isPlausibleSuccessorOf_iff] at h
       obtain ⟨n, hn⟩ := ih
       obtain ⟨a, ha, h₁, h₂, h₃⟩ := h
       refine ⟨n + 1, ?_⟩
@@ -102,59 +68,58 @@ theorem RangeIterator.isPlausibleIndirectOutput_iff'
     induction n generalizing it
     case zero =>
       apply Iter.IsPlausibleIndirectOutput.direct
-      rw [Types.RangeIterator.isPlausibleOutput_iff]
+      rw [RangeIterator.isPlausibleOutput_iff]
       exact ⟨by simpa [LawfulUpwardEnumerable.succMany?_zero] using hn, hu⟩
     case succ ih =>
       cases hn' : it.internalState.next
       · simp [hn'] at hn
       rename_i a
-      simp [hn'] at hn
+      simp only [hn', Option.bind_some] at hn
       have hle : UpwardEnumerable.le a out := ⟨_, hn⟩
       rw [LawfulUpwardEnumerable.succMany?_succ_eq_succ_bind_succMany] at hn
       cases hn' : UpwardEnumerable.succ? a
-      · simp [hn'] at hn
+      · simp only [hn', Option.bind_none, reduceCtorEq] at hn
       rename_i a'
-      simp [hn'] at hn
+      simp only [hn', Option.bind_some] at hn
       specialize ih (it := ⟨some a', it.internalState.upperBound⟩) hn hu
       refine Iter.IsPlausibleIndirectOutput.indirect ?_ ih
-      rw [Types.RangeIterator.isPlausibleSuccessorOf_iff]
+      rw [RangeIterator.isPlausibleSuccessorOf_iff]
       refine ⟨a, ‹_›, ?_, hn', rfl⟩
       apply LawfulUpwardEnumerableUpperBound.isSatisfied_of_le _ a out
       · exact hu
       · exact hle
 
--- TODO: private if it can be accessed via import all
-theorem RangeIterator.isPlausibleIndirectOutput_iff
+theorem Internal.isPlausibleIndirectOutput_iter_iff
     [UpwardEnumerable α] [BoundedUpwardEnumerable sl α]
     [SupportsLowerBound sl α] [SupportsUpperBound su α]
     [LawfulUpwardEnumerable α]
     [LawfulUpwardEnumerableUpperBound su α] [LawfulUpwardEnumerableLowerBound sl α]
     {r : PRange ⟨sl, su⟩ α} {a : α} :
-    r.iterInternal.IsPlausibleIndirectOutput a ↔ a ∈ r := by
-  rw [isPlausibleIndirectOutput_iff']
+    (PRange.Internal.iter r).IsPlausibleIndirectOutput a ↔ a ∈ r := by
+  rw [RangeIterator.isPlausibleIndirectOutput_iff]
   constructor
   · rintro ⟨n, hn, hu⟩
     refine ⟨?_, hu⟩
     rw [LawfulUpwardEnumerableLowerBound.isSatisfied_iff]
-    cases hr : r.iterInternal.internalState.next
+    cases hr : (PRange.Internal.iter r).internalState.next
     · simp [hr] at hn
     rw [hr, Option.bind_some] at hn
     exact ⟨_, hr, n, hn⟩
   · rintro ⟨hl, hu⟩
     rw [LawfulUpwardEnumerableLowerBound.isSatisfied_iff] at hl
     obtain ⟨_, hr, n, hn⟩ := hl
-    exact ⟨n, by simp [PRange.iterInternal, hr, hn], hu⟩
+    exact ⟨n, by simp [PRange.Internal.iter, hr, hn], hu⟩
 
 theorem RangeIterator.upwardEnumerableLe_of_isPlausibleIndirectOutput
     [UpwardEnumerable α] [SupportsUpperBound su α]
     [LawfulUpwardEnumerable α] [LawfulUpwardEnumerableUpperBound su α]
-    {it : Iter (α := Types.RangeIterator su α) α} {out : α}
+    {it : Iter (α := RangeIterator su α) α} {out : α}
     (hout : it.IsPlausibleIndirectOutput out) :
     ∃ a, it.internalState.next = some a ∧ UpwardEnumerable.le a out := by
   have ⟨a, ha⟩ := Option.isSome_iff_exists.mp <|
-    Types.RangeIterator.isSome_next_of_isPlausibleIndirectOutput hout
+    RangeIterator.isSome_next_of_isPlausibleIndirectOutput hout
   refine ⟨a, ha, ?_⟩
-  simp only [isPlausibleIndirectOutput_iff', ha, Option.bind_some, exists_and_right] at hout
+  simp only [isPlausibleIndirectOutput_iff, ha, Option.bind_some, exists_and_right] at hout
   exact hout.1
 
 @[no_expose]
@@ -162,26 +127,28 @@ instance [UpwardEnumerable α] [BoundedUpwardEnumerable sl α]
     [SupportsLowerBound sl α] [SupportsUpperBound su α]
     [LawfulUpwardEnumerable α]
     [LawfulUpwardEnumerableLowerBound sl α] [LawfulUpwardEnumerableUpperBound su α]
-    [Monad m] [Finite (Types.RangeIterator su α) Id] :
+    [Monad m] [Finite (RangeIterator su α) Id] :
     ForIn' m (PRange ⟨sl, su⟩ α) α inferInstance where
   forIn' r init f := by
     haveI : MonadLift Id m := ⟨Std.Internal.idToMonad (α := _)⟩
-    haveI := Iter.instForIn' (α := Types.RangeIterator su α) (β := α) (n := m)
-    refine ForIn'.forIn' (α := α) r.iterInternal init (fun a ha acc => f a ?_ acc)
+    haveI := Iter.instForIn' (α := RangeIterator su α) (β := α) (n := m)
+    refine ForIn'.forIn' (α := α) (PRange.Internal.iter r) init (fun a ha acc => f a ?_ acc)
     simp only [Membership.mem] at ha
-    rwa [RangeIterator.isPlausibleIndirectOutput_iff] at ha
+    rwa [PRange.Internal.isPlausibleIndirectOutput_iter_iff] at ha
 
 end Iterator
 
-theorem Range.mem.upper [LE α] [DecidableLE α] {i : α} {r : PRange ⟨.unbounded, .closed⟩ α} (h : i ∈ r) : i ≤ r.upper :=
+theorem PRange.mem.upper [LE α] [DecidableLE α] {i : α} {r : PRange ⟨.unbounded, .closed⟩ α} (h : i ∈ r) : i ≤ r.upper :=
   h.2
 
 -- theorem Range.mem.lower [LE α] {i : α} {r : PRange ⟨.unbounded, .closed⟩ α} (h : i ∈ r) : r.lower ≤ i := h.1
 
 -- theorem Range.mem.step {i : Nat} {r : PRange shape α} (h : i ∈ r) : (i - r.start) % r.step = 0 := h.2.2
 
-theorem Range.get_elem_helper {i n : Nat} {r : PRange ⟨.closed, .open⟩ Nat} (h₁ : i ∈ r) (h₂ : r.upper = n) :
+theorem PRange.get_elem_helper {i n : Nat} {r : PRange ⟨.closed, .open⟩ Nat} (h₁ : i ∈ r) (h₂ : r.upper = n) :
     i < n := h₂ ▸ h₁.2
 
 macro_rules
   | `(tactic| get_elem_tactic_extensible) => `(tactic| apply Range.get_elem_helper; assumption; rfl)
+
+end Std.PRange
