src/Init/Data/Range/Polymorphic/Lemmas.lean
@@ -17,33 +17,33 @@ open Std.Iterators
 
 variable {shape : RangeShape} {α : Type u}
 
-private theorem iterInternal_open_eq_of_isSome_succ? [UpwardEnumerable α]
+private theorem Internal.iter_open_eq_of_isSome_succ? [UpwardEnumerable α]
     [SupportsUpperBound su α] [HasFiniteRanges su α]
     [LawfulUpwardEnumerable α]
     {lo : Bound .open α} {hi} (h : (UpwardEnumerable.succ? lo).isSome) :
-    (PRange.mk (shape := ⟨.open, su⟩) lo hi).iterInternal =
-      (PRange.mk (shape := ⟨.closed, su⟩) (UpwardEnumerable.succ? lo |>.get h) hi).iterInternal := by
-  simp [PRange.iterInternal, BoundedUpwardEnumerable.init?]
+    Internal.iter (PRange.mk (shape := ⟨.open, su⟩) lo hi) =
+      Internal.iter (PRange.mk (shape := ⟨.closed, su⟩) (UpwardEnumerable.succ? lo |>.get h) hi) := by
+  simp [Internal.iter, BoundedUpwardEnumerable.init?]
 
-private theorem toList_eq_toList_iterInternal [UpwardEnumerable α]
+private theorem toList_eq_toList_internalIter [UpwardEnumerable α]
     [BoundedUpwardEnumerable sl α] [SupportsUpperBound su α] [HasFiniteRanges su α]
     [LawfulUpwardEnumerable α]
     {r : PRange ⟨sl, su⟩ α} :
-    r.toList = r.iterInternal.toList := by
+    r.toList = (Internal.iter r).toList := by
   rfl
 
 theorem toList_eq_match [UpwardEnumerable α]
     [SupportsUpperBound su α] [HasFiniteRanges su α]
     [LawfulUpwardEnumerable α]
-    {it : Iter (α := Types.RangeIterator su α) α} :
+    {it : Iter (α := RangeIterator su α) α} :
     it.toList =  match it.internalState.next with
       | none => []
       | some a => if SupportsUpperBound.IsSatisfied it.internalState.upperBound a then
-          a :: (⟨⟨UpwardEnumerable.succ? a, it.internalState.upperBound⟩⟩ : Iter (α := Types.RangeIterator su α) α).toList
+          a :: (⟨⟨UpwardEnumerable.succ? a, it.internalState.upperBound⟩⟩ : Iter (α := RangeIterator su α) α).toList
         else
           [] := by
-  rw [Iter.toList_eq_match_step, Types.RangeIterator.step_eq_step]
-  simp only [Types.RangeIterator.step, PRange.iterInternal]
+  rw [Iter.toList_eq_match_step, RangeIterator.step_eq_step]
+  simp only [RangeIterator.step, Internal.iter]
   split <;> rename_i heq <;> simp only [Subtype.mk.injEq] at heq
   · split at heq <;> rename_i heq'
     · cases heq
@@ -63,10 +63,10 @@ theorem toList_eq_aux [UpwardEnumerable α]
         a :: (PRange.mk (shape := ⟨.open, su⟩) a r.upper).toList
       else
         [] := by
-  simp only [PRange.toList_eq_toList_iterInternal,
-    show r.upper = r.iterInternal.internalState.upperBound by rfl,
-    show UpwardEnumerable.succ? r.lower = r.iterInternal.internalState.next by rfl]
-  generalize r.iterInternal = it
+  simp only [PRange.toList_eq_toList_internalIter,
+    show r.upper = (Internal.iter r).internalState.upperBound by rfl,
+    show UpwardEnumerable.succ? r.lower = (Internal.iter r).internalState.next by rfl]
+  generalize Internal.iter r = it
   rw [toList_eq_match]
   split
   · simp_all
@@ -84,13 +84,13 @@ theorem toList_eq [UpwardEnumerable α] [BoundedUpwardEnumerable sl α]
         a :: (PRange.mk (shape := ⟨.open, su⟩) a r.upper).toList
       else
         [] := by
-  rw [toList_eq_toList_iterInternal, toList_eq_match,
-    show r.iterInternal.internalState.next = BoundedUpwardEnumerable.init? r.lower by rfl,
-    show r.iterInternal.internalState.upperBound = r.upper by rfl]
+  rw [toList_eq_toList_internalIter, toList_eq_match,
+    show (Internal.iter r).internalState.next = BoundedUpwardEnumerable.init? r.lower by rfl,
+    show (Internal.iter r).internalState.upperBound = r.upper by rfl]
   split
   · rfl
   · split
-    · simp only [List.cons.injEq, true_and, toList_eq_toList_iterInternal, PRange.iterInternal,
+    · simp only [List.cons.injEq, true_and, toList_eq_toList_internalIter, Internal.iter,
         BoundedUpwardEnumerable.init?]
     · rfl
 
@@ -100,7 +100,7 @@ private theorem toList_open_eq_of_isSome_succ? [UpwardEnumerable α]
     {lo : Bound .open α} {hi} (h : (UpwardEnumerable.succ? lo).isSome) :
     (PRange.mk (shape := ⟨.open, su⟩) lo hi).toList =
       (PRange.mk (shape := ⟨.closed, su⟩) (UpwardEnumerable.succ? lo |>.get h) hi).toList := by
-  simp [toList_eq_toList_iterInternal, iterInternal_open_eq_of_isSome_succ?, h]
+  simp [toList_eq_toList_internalIter, Internal.iter_open_eq_of_isSome_succ?, h]
 
 theorem toList_eq_nil_iff [UpwardEnumerable α]
     [SupportsUpperBound su α] [HasFiniteRanges su α] [BoundedUpwardEnumerable sl α]
@@ -108,8 +108,8 @@ theorem toList_eq_nil_iff [UpwardEnumerable α]
     {r : PRange ⟨sl, su⟩ α} :
     r.toList = [] ↔
       ¬ (∃ a, BoundedUpwardEnumerable.init? r.lower = some a ∧ SupportsUpperBound.IsSatisfied r.upper a) := by
-  rw [toList_eq_toList_iterInternal] --, Iter.toList_eq_match_step, Types.RangeIterator.step_eq_step]
-  rw [toList_eq_match, PRange.iterInternal]
+  rw [toList_eq_toList_internalIter] --, Iter.toList_eq_match_step, RangeIterator.step_eq_step]
+  rw [toList_eq_match, Internal.iter]
   simp only
   split <;> rename_i heq <;> simp [heq]
 
@@ -119,18 +119,18 @@ theorem RangeIterator.mem_toList_iff_isPlausibleIndirectOutput
     [LawfulUpwardEnumerable α]
     [LawfulUpwardEnumerableUpperBound su α]
     [HasFiniteRanges su α]
-    {it : Iter (α := Types.RangeIterator su α) α} :
+    {it : Iter (α := RangeIterator su α) α} :
     out ∈ it.toList ↔ it.IsPlausibleIndirectOutput out := by
   constructor
   · apply Iter.isPlausibleIndirectOutput_of_mem_toList
   · intro h
     induction h
     · rename_i it out h
-      rw [Types.RangeIterator.isPlausibleOutput_iff] at h
+      rw [RangeIterator.isPlausibleOutput_iff] at h
       rw [toList_eq_match]
       simp [h]
     · rename_i it it' out h _ h'
-      rw [Types.RangeIterator.isPlausibleSuccessorOf_iff] at h
+      rw [RangeIterator.isPlausibleSuccessorOf_iff] at h
       obtain ⟨a, ha⟩ := h
       rw [toList_eq_match]
       simp only [ha.1, ha.2.1, ha.2.2.1]
@@ -140,7 +140,7 @@ instance [UpwardEnumerable α]
     [SupportsUpperBound su α] [HasFiniteRanges su α]
     [LawfulUpwardEnumerable α]
     [LawfulUpwardEnumerableUpperBound su α] :
-    LawfulPureIterator (Types.RangeIterator su α) where
+    LawfulPureIterator (RangeIterator su α) where
   mem_toList_iff_isPlausibleIndirectOutput :=
     RangeIterator.mem_toList_iff_isPlausibleIndirectOutput
 
@@ -150,8 +150,8 @@ theorem mem_toList_iff_mem [UpwardEnumerable α]
     [LawfulUpwardEnumerableLowerBound sl α] [LawfulUpwardEnumerableUpperBound su α]
     {r : PRange ⟨sl, su⟩ α}
     {a : α} : a ∈ r.toList ↔ a ∈ r := by
-  rw [toList_eq_toList_iterInternal, RangeIterator.mem_toList_iff_isPlausibleIndirectOutput,
-    RangeIterator.isPlausibleIndirectOutput_iff]
+  rw [toList_eq_toList_internalIter, RangeIterator.mem_toList_iff_isPlausibleIndirectOutput,
+    Internal.isPlausibleIndirectOutput_iter_iff]
 
 theorem pairwise_upwardEnumerableLt [UpwardEnumerable α]
     [SupportsUpperBound su α] [SupportsLowerBound sl α] [HasFiniteRanges su α]
@@ -159,8 +159,8 @@ theorem pairwise_upwardEnumerableLt [UpwardEnumerable α]
     [LawfulUpwardEnumerableLowerBound sl α] [LawfulUpwardEnumerableUpperBound su α]
     {r : PRange ⟨sl, su⟩ α} :
     r.toList.Pairwise (fun a b => UpwardEnumerable.lt a b) := by
-  rw [PRange.toList_eq_toList_iterInternal]
-  generalize r.iterInternal = it
+  rw [PRange.toList_eq_toList_internalIter]
+  generalize Internal.iter r = it
   induction it using Iter.inductSteps with | step it ihy ihs =>
   rw [toList_eq_match]
   repeat' split <;> (try exact .nil; done)
@@ -177,17 +177,17 @@ theorem pairwise_upwardEnumerableLt [UpwardEnumerable α]
       exact ha.choose_spec.1
     exact UpwardEnumerable.lt_of_lt_of_le this ha.choose_spec.2
   · apply ihy (out := a)
-    simp_all [Types.RangeIterator.isPlausibleStep_iff, Types.RangeIterator.step]
+    simp_all [RangeIterator.isPlausibleStep_iff, RangeIterator.step]
 
-theorem forIn'_eq_forIn'_iterInternal [UpwardEnumerable α]
+theorem forIn'_eq_forIn'_internalIter [UpwardEnumerable α]
     [SupportsUpperBound su α] [SupportsLowerBound sl α] [HasFiniteRanges su α]
     [BoundedUpwardEnumerable sl α] [LawfulUpwardEnumerable α]
     [LawfulUpwardEnumerableLowerBound sl α] [LawfulUpwardEnumerableUpperBound su α]
     {r : PRange ⟨sl, su⟩ α}
     {γ : Type u} {init : γ} {m : Type u → Type w} [Monad m] {f : (a : α) → a ∈ r → γ → m (ForInStep γ)} :
-    haveI := Iter.instForIn' (α := Types.RangeIterator su α) (β := α) (n := m)
+    haveI := Iter.instForIn' (α := RangeIterator su α) (β := α) (n := m)
     ForIn'.forIn' r init f =
-      ForIn'.forIn' r.iterInternal init (fun a ha acc => f a (RangeIterator.isPlausibleIndirectOutput_iff.mp ha) acc) := by
+      ForIn'.forIn' (Internal.iter r) init (fun a ha acc => f a (Internal.isPlausibleIndirectOutput_iter_iff.mp ha) acc) := by
   rfl
 
 theorem forIn'_eq_forIn'_toList [UpwardEnumerable α]
@@ -199,7 +199,7 @@ theorem forIn'_eq_forIn'_toList [UpwardEnumerable α]
     {f : (a : α) → a ∈ r → γ → m (ForInStep γ)} :
     ForIn'.forIn' r init f =
       ForIn'.forIn' r.toList init (fun a ha acc => f a (mem_toList_iff_mem.mp ha) acc) := by
-  simp [forIn'_eq_forIn'_iterInternal, toList_eq_toList_iterInternal,
+  simp [forIn'_eq_forIn'_internalIter, toList_eq_toList_internalIter,
     Iter.forIn'_eq_forIn'_toList]
 
 theorem forIn'_toList_eq_forIn' [UpwardEnumerable α]
@@ -241,8 +241,8 @@ theorem forIn'_eq_match [UpwardEnumerable α]
         | .done c => return c
       else
         return init := by
-  rw [forIn'_eq_forIn'_iterInternal, Iter.forIn'_eq_match_step]
-  simp only [Types.RangeIterator.step_eq_step, Types.RangeIterator.step, PRange.iterInternal]
+  rw [forIn'_eq_forIn'_internalIter, Iter.forIn'_eq_match_step]
+  simp only [RangeIterator.step_eq_step, RangeIterator.step, Internal.iter]
   apply Eq.symm
   split <;> rename_i heq
   · simp [heq]
@@ -252,7 +252,7 @@ theorem forIn'_eq_match [UpwardEnumerable α]
       apply bind_congr
       intro step
       split
-      · simp [forIn'_eq_forIn'_iterInternal, PRange.iterInternal, BoundedUpwardEnumerable.init?]
+      · simp [forIn'_eq_forIn'_internalIter, Internal.iter, BoundedUpwardEnumerable.init?]
       · simp
     · simp
 
